restructuring of rsapss modules

code/experimental/rsapss/spec/Spec.RSA.Lemmas.fst
@@ -6,7 +6,6 @@ open FStar.Math.Lemmas
 open Lib.IntTypes
 open Spec.Bignum.Basic
 
-(* LEMMAS *)
 #reset-options "--z3rlimit 30 --max_fuel 2"
 val pow : x:nat -> n:nat -> Tot nat
 let rec pow x n =
@@ -73,71 +72,6 @@ let lemma_mod_mult_div a b d n =
 val lemma_mul_div_mod:a:nat -> b:pos -> c:nat -> d:pos -> e:pos -> n:pos
   -> Lemma (((a / b) * (c / d)) / e % n == a * c / (b * d * e) % n)
 let lemma_mul_div_mod a b c d e n = admit()
-
-(* Lemmas for Montgomery's arithmetic *)
-val lemma_mont_reduction_f:
-    #nBits:size_pos
-  -> #cBits:size_pos
-  -> rBits:size_pos{nBits < rBits /\ nBits + 1 + rBits < max_size_t}
-  -> n:bignum nBits{bn_v n > 0}
-  -> c:bignum cBits{cBits < nBits + rBits}
-  -> i:size_nat{64 * (i + 1) <= rBits}
-  -> Lemma
-    (requires True)
-    (ensures
-      bn_v c + (pow2 (64 * (i + 1)) - 1) * bn_v n < pow2 (nBits + 1 + rBits))
-let lemma_mont_reduction_f #nBits #cBits rBits n c i =
-  pow2_le_compat rBits (64 * (i + 1));
-  assert (bn_v c + (pow2 (64 * (i + 1)) - 1) * bn_v n < pow2 cBits + pow2 rBits * pow2 nBits);
-  pow2_plus rBits nBits;
-  pow2_lt_compat (nBits + rBits) cBits;
-  assert (bn_v c + (pow2 (64 * (i + 1)) - 1) * bn_v n < pow2 (nBits + rBits) + pow2 (nBits + rBits));
-  pow2_double_sum (nBits + rBits)
-
-val lemma_mont_reduction:
-    #nBits:size_pos
-  -> #cBits:size_pos
-  -> rBits:size_pos{nBits < rBits /\ nBits+1+rBits < max_size_t}
-  -> n:bignum nBits{bn_v n > 0}
-  -> c:bignum cBits{cBits < nBits + rBits}
-  -> Lemma
-    (requires True)
-    (ensures  bn_v c + (pow2 rBits - 1) * bn_v n < pow2 (nBits + 1 + rBits))
-let lemma_mont_reduction #nBits #cBits rBits n c =
-  assert (bn_v c + (pow2 rBits - 1) * bn_v n < pow2 cBits + pow2 rBits * pow2 nBits);
-  pow2_plus rBits nBits;
-  pow2_lt_compat (nBits + rBits) cBits;
-  assert (bn_v c + (pow2 rBits - 1) * bn_v n < pow2 (nBits + rBits) + pow2 (nBits + rBits));
-  pow2_double_sum (nBits + rBits)
-
-val lemma_mont_reduction_fi:
-    #nBits:size_pos
-  -> #cBits:size_pos
-  -> rBits:size_pos{nBits < rBits /\ nBits + 1 + rBits < max_size_t}
-  -> qi:bignum 64
-  -> n:bignum nBits{bn_v n > 0}
-  -> c:bignum cBits
-  -> i:size_nat{i <= rBits / 64}
-  -> res:bignum (nBits + 1 + rBits)
-  -> Lemma
-    (requires
-      bn_v res + bn_v n * pow2 (64 * i) * bn_v qi <=
-      bn_v c + (pow2 (64 * i) - 1) * bn_v n + bn_v n * pow2 (64 * i) * bn_v qi)
-    (ensures
-      bn_v res + bn_v n * pow2 (64 * i) * bn_v qi <=
-      bn_v c + (pow2 (64 * (i + 1)) - 1) * bn_v n)
-let lemma_mont_reduction_fi #nBits #cBits rBits qi n c i res =
-  let res1 = bn_v res + bn_v n * pow2 (64 * i) * bn_v qi in
-  assert (res1 <= bn_v c + (pow2 (64 * i) - 1) * bn_v n + bn_v n * pow2 (64 * i) * bn_v qi); //from ind hypo
-  assert (bn_v qi < pow2 64);
-  FStar.Math.Lemmas.lemma_mult_le_right (bn_v n * pow2 (64 * i)) (bn_v qi) (pow2 64 - 1);
-  assert (res1 <= bn_v c + (pow2 (64 * i) - 1) * bn_v n + bn_v n * pow2 (64 * i) * (pow2 64 - 1));
-  assert (res1 <= bn_v c + pow2 (64 * i) * bn_v n - bn_v n + bn_v n * pow2 (64 * i) * (pow2 64 - 1));
-  assert (res1 <= bn_v c + pow2 (64 * i) * bn_v n - bn_v n + bn_v n * pow2 (64 * i) * pow2 64 - bn_v n * pow2 (64 * i));
-  assert (res1 <= bn_v c - bn_v n + bn_v n * pow2 (64 * i) * pow2 64);
-  assert (res1 <= bn_v c + (pow2 (64 * i) * pow2 64 - 1) * bn_v n);
-  pow2_plus (64 * i) 64;
-  assert (res1 <= bn_v c + (pow2 (64 * (i + 1)) - 1) * bn_v n)
 
 (* LEMMAS for modular exponentiation *)
 assume
