code/experimental/rsapss/spec/Spec.Montgomery.Lemmas.fst
@@ -1,0 +1,78 @@
+module Spec.Montgomery.Lemmas
+
+open FStar.Mul
+open FStar.Math.Lemmas
+
+open Lib.IntTypes
+open Spec.Bignum.Basic
+
+#reset-options "--z3rlimit 30 --max_fuel 0 --max_ifuel 0"
+
+// (1 / d) % n is an inverse element of d
+val lemma_mod_mult_div_1:a:nat -> d:pos -> n:pos
+  -> Lemma (a / d % n == (a % n) / d % n)
+let lemma_mod_mult_div_1 a d n = admit()
+
+val lemma_mont_reduction_f:
+    #nBits:size_pos
+  -> #cBits:size_pos
+  -> rBits:size_pos{nBits < rBits /\ nBits + 1 + rBits < max_size_t}
+  -> n:bignum nBits{bn_v n > 0}
+  -> c:bignum cBits{cBits < nBits + rBits}
+  -> i:size_nat{64 * (i + 1) <= rBits}
+  -> Lemma
+    (requires True)
+    (ensures
+      bn_v c + (pow2 (64 * (i + 1)) - 1) * bn_v n < pow2 (nBits + 1 + rBits))
+let lemma_mont_reduction_f #nBits #cBits rBits n c i =
+  pow2_le_compat rBits (64 * (i + 1));
+  assert (bn_v c + (pow2 (64 * (i + 1)) - 1) * bn_v n < pow2 cBits + pow2 rBits * pow2 nBits);
+  pow2_plus rBits nBits;
+  pow2_lt_compat (nBits + rBits) cBits;
+  assert (bn_v c + (pow2 (64 * (i + 1)) - 1) * bn_v n < pow2 (nBits + rBits) + pow2 (nBits + rBits));
+  pow2_double_sum (nBits + rBits)
+
+val lemma_mont_reduction:
+    #nBits:size_pos
+  -> #cBits:size_pos
+  -> rBits:size_pos{nBits < rBits /\ nBits+1+rBits < max_size_t}
+  -> n:bignum nBits{bn_v n > 0}
+  -> c:bignum cBits{cBits < nBits + rBits}
+  -> Lemma
+    (requires True)
+    (ensures  bn_v c + (pow2 rBits - 1) * bn_v n < pow2 (nBits + 1 + rBits))
+let lemma_mont_reduction #nBits #cBits rBits n c =
+  assert (bn_v c + (pow2 rBits - 1) * bn_v n < pow2 cBits + pow2 rBits * pow2 nBits);
+  pow2_plus rBits nBits;
+  pow2_lt_compat (nBits + rBits) cBits;
+  assert (bn_v c + (pow2 rBits - 1) * bn_v n < pow2 (nBits + rBits) + pow2 (nBits + rBits));
+  pow2_double_sum (nBits + rBits)
+
+val lemma_mont_reduction_fi:
+    #nBits:size_pos
+  -> #cBits:size_pos
+  -> rBits:size_pos{nBits < rBits /\ nBits + 1 + rBits < max_size_t}
+  -> qi:bignum 64
+  -> n:bignum nBits{bn_v n > 0}
+  -> c:bignum cBits
+  -> i:size_nat{i <= rBits / 64}
+  -> res:bignum (nBits + 1 + rBits)
+  -> Lemma
+    (requires
+      bn_v res + bn_v n * pow2 (64 * i) * bn_v qi <=
+      bn_v c + (pow2 (64 * i) - 1) * bn_v n + bn_v n * pow2 (64 * i) * bn_v qi)
+    (ensures
+      bn_v res + bn_v n * pow2 (64 * i) * bn_v qi <=
+      bn_v c + (pow2 (64 * (i + 1)) - 1) * bn_v n)
+let lemma_mont_reduction_fi #nBits #cBits rBits qi n c i res =
+  let res1 = bn_v res + bn_v n * pow2 (64 * i) * bn_v qi in
+  assert (res1 <= bn_v c + (pow2 (64 * i) - 1) * bn_v n + bn_v n * pow2 (64 * i) * bn_v qi); //from ind hypo
+  assert (bn_v qi < pow2 64);
+  FStar.Math.Lemmas.lemma_mult_le_right (bn_v n * pow2 (64 * i)) (bn_v qi) (pow2 64 - 1);
+  assert (res1 <= bn_v c + (pow2 (64 * i) - 1) * bn_v n + bn_v n * pow2 (64 * i) * (pow2 64 - 1));
+  assert (res1 <= bn_v c + pow2 (64 * i) * bn_v n - bn_v n + bn_v n * pow2 (64 * i) * (pow2 64 - 1));
+  assert (res1 <= bn_v c + pow2 (64 * i) * bn_v n - bn_v n + bn_v n * pow2 (64 * i) * pow2 64 - bn_v n * pow2 (64 * i));
+  assert (res1 <= bn_v c - bn_v n + bn_v n * pow2 (64 * i) * pow2 64);
+  assert (res1 <= bn_v c + (pow2 (64 * i) * pow2 64 - 1) * bn_v n);
+  pow2_plus (64 * i) 64;
+  assert (res1 <= bn_v c + (pow2 (64 * (i + 1)) - 1) * bn_v n)
